- progression preuve Isabelle - corrections async_to_stab

proof_Isabelle/sync-mod/GenSynchMod.thy
@@ -54,7 +54,7 @@ definition gen_nextState :: "Proc => locState => (Proc => locState message) => l
         else
             conc s' = isConc msgs & ready s' = isReady msgs)
     else
-        x s' = 0 & forc s' = (if ready_level1 msgs s then 1 else 2) & level s' = forc s' & ready s' = (level s' > 0) & conc s'"
+        x s' = 0 & level s' = (if ready_level1 msgs s then 1 else 2) & forc s' = max (level s') (maxForce msgs) & ready s' = (level s' > 0) & conc s'"
 
 definition gen_sendMsg where
 "gen_sendMsg p q st == st"
